Clean.lean
@@ -41,4 +41,5 @@ import Clean.Gadgets.BLAKE3.FinalStateUpdate
 import Clean.Gadgets.BLAKE3.Round
 import Clean.Gadgets.BLAKE3.FinalizeChunk
 import Clean.Examples.FibonacciVm.Circuit
+import Clean.Examples.FibonacciNextRow
 import Clean.Gadgets.SHA256.SHA256Compress
